CertifyingDatalog/GraphValidation.lean
@@ -4,6 +4,7 @@ import CertifyingDatalog.TreeValidation
 import Mathlib.Data.List.Card
 import Mathlib.Data.Finset.Card
 
+
 structure Graph (A: Type) where
   (vertices: List A)
   (predecessors: A → List A)
@@ -20,12 +21,28 @@ def isPath (l: List A) (G: Graph A): Prop :=
     | hd'::tl' =>
       hd ∈ G.vertices ∧ hd ∈ (G.predecessors hd') ∧ isPath (hd'::tl') G
 
+lemma singletonPath (a:A) (G: Graph A) (mem: a ∈ G.vertices): isPath [a] G :=
+by
+  unfold isPath
+  simp
+  apply mem
+
 def List.getFirst (l: List A) (nonempty: l ≠ []): A :=
   match l with
   | [] => have f: False := by
             simp at nonempty
     False.elim f
   | hd::_ => hd
+
+def List.getLast' (l: List A) (nonempty: l ≠ []): A :=
+  match l with
+  | [] => have f: False := by
+            simp at nonempty
+    False.elim f
+  | hd::tl =>
+    if h:tl = []
+    then hd
+    else List.getLast' tl h
 
 def isCircle (l: List A) (G: Graph A): Prop :=
   if h:List.length l < 2
@@ -39,10 +56,22 @@ def isCircle (l: List A) (G: Graph A): Prop :=
       | cons hd tl =>
         simp
 
-    isPath l G ∧ List.getLast l l_nonempty = List.getFirst l l_nonempty
+    isPath l G ∧ List.getLast' l l_nonempty = List.getFirst l l_nonempty
 
 
 def isAcyclic (G: Graph A) := ∀ (l: List A), ¬ isCircle l G
+
+lemma isPath_of_cons {a: A} {l:List A} {G:Graph A} (path: isPath (a::l) G): isPath l G :=
+by
+  unfold isPath at path
+  cases l with
+  | nil =>
+    unfold isPath
+    apply True.intro
+  | cons hd tl =>
+    simp at path
+    simp [path]
+
 
 lemma removeFrontOfLtMin (a b c: ℕ) (hab: b ≤ a) (hac: c ≤ a) : a - b < a -c ↔ b > c :=
 by
@@ -70,8 +99,6 @@ by
         rw [Nat.succ_lt_succ_iff]
 
 
-
-
 lemma isPath_front_member_graph{a: A} {l: List A} {G: Graph A} (path: isPath (a::l) G): a ∈ G.vertices :=
 by
   cases l with
@@ -83,6 +110,22 @@ by
     unfold isPath at path
     simp at path
     simp [path]
+
+lemma isPath_member_graph {a: A} {l: List A} {G: Graph A} (path: isPath l G) (mem: a ∈ l): a ∈ G.vertices :=
+by
+  induction l with
+  | nil =>
+    simp at mem
+  | cons hd tl ih =>
+    simp at mem
+    cases mem with
+    | inl a_hd =>
+      rw [← a_hd] at path
+      apply isPath_front_member_graph path
+    | inr a_tl =>
+      apply ih
+      apply isPath_of_cons path
+      apply a_tl
 
 lemma isPath_extends_predecessors {a: A} {l: List A} {G: Graph A} (path: isPath (a::l) G): ∀ (b:A), b ∈ (G.predecessors a) → isPath (b::a::l) G :=
 by
@@ -97,18 +140,6 @@ by
   apply b_mem
   apply path
 
-
-
-lemma isPath_of_cons {a: A} {l:List A} {G:Graph A} (path: isPath (a::l) G): isPath l G :=
-by
-  unfold isPath at path
-  cases l with
-  | nil =>
-    unfold isPath
-    apply True.intro
-  | cons hd tl =>
-    simp at path
-    simp [path]
 
 lemma isPathImplSubset {l: List A} {G: Graph A} (path: isPath l G ): l.toFinset ⊆ G.vertices.toFinset :=
 by
@@ -164,3 +195,283 @@ decreasing_by
   apply Finset.card_le_of_subset
   apply isPathImplSubset
   apply isPath_of_cons path
+
+lemma extractTreeStepHeight (a ga:A) (G:Graph A) (visited: List A) (path: isPath (a::visited) G) (neighbor: ga ∈ G.predecessors a) (a_vis: ¬ a ∈ visited): height (extractTreeStep a G visited path) > height (extractTreeStep ga G (a::visited) (isPath_extends_predecessors path ga neighbor)) :=
+by
+  simp
+  apply heightOfMemberIsSmaller
+  -- to avoid unnecessary unfolding
+  generalize h:(extractTreeStep ga G (a :: visited) (_ : isPath (ga :: a :: visited) G)) = t
+  unfold extractTreeStep
+  simp [a_vis]
+  unfold member
+  simp
+  use ga
+  use neighbor
+
+lemma rootOfExtractTreeStep (a:A) (G:Graph A) (visited: List A) (path: isPath (a::visited) G): root (extractTreeStep a G visited path) = a :=
+by
+  unfold extractTreeStep
+  unfold root
+  by_cases a_visited: a ∈ visited
+  simp [a_visited]
+  simp [a_visited]
+
+def getSubListToMember (l: List A) (a: A) (mem: a ∈ l): List A :=
+  match l with
+  | [] =>
+    have h: False :=
+    by
+      simp at mem
+
+    False.elim h
+  | hd::tl =>
+    if p: a = hd
+    then [hd]
+    else
+      have mem': a ∈ tl :=
+      by
+        simp[p] at mem
+        apply mem
+      hd::getSubListToMember tl a mem'
+
+lemma getSubListToMemberPreservesFront (hd a hd': A) (tl tl': List A) (mem: a ∈ hd'::tl') (result: getSubListToMember (hd'::tl') a mem = hd::tl): hd' = hd :=
+by
+  unfold getSubListToMember at result
+  by_cases a_hd: a = hd'
+  all_goals{
+  simp [a_hd] at result
+  simp [result]
+  }
+
+
+
+lemma getSubListToMemberPreservesPath (l: List A) (a:A) (mem: a ∈ l) (G: Graph A) (path: isPath l G): isPath (getSubListToMember l a mem) G :=
+by
+  induction l with
+  | nil =>
+    simp at mem
+  | cons hd tl ih =>
+    unfold getSubListToMember
+    by_cases a_hd: a = hd
+    simp [a_hd]
+    unfold isPath
+    simp
+    apply isPath_front_member_graph path
+
+
+    simp[a_hd]
+    unfold isPath
+    cases tl with
+    | nil =>
+      simp [a_hd] at mem
+    | cons hd' tl' =>
+      unfold getSubListToMember
+      by_cases a_hd': a = hd'
+      simp [a_hd']
+      unfold isPath
+      simp
+      constructor
+      apply isPath_member_graph
+      apply path
+      simp
+
+      unfold isPath at path
+      simp at path
+      simp [path]
+      rcases path with ⟨_,_, path_hd'_tl'⟩
+      apply isPath_member_graph path_hd'_tl'
+      simp
+
+      simp [a_hd']
+      rw [List.mem_cons] at mem
+      cases mem with
+      | inl h =>
+        exact absurd h a_hd
+      | inr h =>
+        specialize ih h
+        unfold isPath at path
+        simp at path
+        rcases path with ⟨hd_G,hd_hd', path_hd'_tl'⟩
+        specialize ih path_hd'_tl'
+        constructor
+        apply hd_G
+        constructor
+        apply hd_hd'
+        unfold getSubListToMember  at ih
+        simp [a_hd'] at ih
+        apply ih
+
+
+lemma getSubListToMemberIsNotEmpty (l: List A) (a:A) (mem: a ∈ l): getSubListToMember l a mem ≠ [] :=
+by
+  unfold getSubListToMember
+  cases l with
+  | nil =>
+    simp at mem
+  | cons hd tl =>
+    simp
+    by_cases a_hd: a=hd
+    simp [a_hd]
+    simp [a_hd]
+
+
+lemma getSubListToMemberGetLastIsMember (l: List A) (a:A) (mem: a ∈ l): (getSubListToMember l a mem).getLast' (getSubListToMemberIsNotEmpty l a mem) = a :=
+by
+  induction l with
+  | nil =>
+    simp at mem
+  | cons hd tl ih =>
+    unfold getSubListToMember
+    by_cases a_hd: a=hd
+    simp [a_hd]
+    unfold List.getLast'
+    simp
+
+    simp[a_hd]
+    unfold List.getLast'
+    simp[a_hd] at mem
+    have h: getSubListToMember tl a mem ≠ []
+    apply getSubListToMemberIsNotEmpty
+    simp [h]
+    apply ih
+
+lemma frontRepetitionInPathImpliesCircle (a:A) (G:Graph A) (visited: List A) (path: isPath (a::visited) G) (mem: a ∈ visited): isCircle (a::(getSubListToMember visited a mem)) G :=
+by
+  unfold isCircle
+  simp
+  have not_p: ¬ getSubListToMember visited a mem = []
+  apply getSubListToMemberIsNotEmpty
+  have h: ¬ Nat.succ (List.length (getSubListToMember visited a mem)) < 2
+  simp
+  rw [Nat.two_le_iff]
+  simp
+  by_contra p
+  rw [List.length_eq_zero] at p
+
+  exact absurd p not_p
+
+  simp [h]
+  constructor
+  unfold isPath
+  cases p: getSubListToMember visited a mem with
+  | nil =>
+    exact absurd p not_p
+  | cons hd tl =>
+    simp
+    unfold isPath at path
+    cases q:visited with
+    | nil =>
+      simp[q] at mem
+    | cons hd' tl' =>
+      simp[q] at path
+      simp [q] at p
+      have hd_hd': hd' = hd
+      apply getSubListToMemberPreservesFront
+      apply p
+      rw [← hd_hd']
+      simp [path]
+      rw [hd_hd', ← p]
+      apply getSubListToMemberPreservesPath
+      simp [path]
+
+  unfold List.getFirst
+  unfold List.getLast'
+  simp [not_p]
+  rw [getSubListToMemberGetLastIsMember]
+
+
+
+
+variable {τ: signature} [DecidableEq τ.vars] [DecidableEq τ.constants] [DecidableEq τ.relationSymbols] [Inhabited τ.constants]
+
+def locallyValid (P: program τ) (d: database τ) (v: groundAtom τ) (G: Graph (groundAtom τ)): Prop :=
+ (∃(r: rule τ) (g:grounding τ), r ∈ P ∧ ruleGrounding r g = groundRuleFromAtoms v (G.predecessors v) ) ∨ ((G.predecessors v) = [] ∧ d.contains v)
+
+lemma extractTreeStepValidProofTreeIffAllLocallyValidAndAcyclic (P: program τ) (d: database τ) (a: groundAtom τ) (G: Graph (groundAtom τ)) (acyclic: isAcyclic G) (visited: List (groundAtom τ)) (path: isPath (a::visited) G) (valid: ∀ (a: groundAtom τ), a ∈ G.vertices → locallyValid P d a G): isValid P d (extractTreeStep a G visited path) :=
+by
+  induction' h:(height (extractTreeStep a G visited path)) using Nat.strongInductionOn with n ih generalizing a visited
+  unfold extractTreeStep
+
+  have a_visited: ¬ a ∈ visited
+  by_contra p
+  have circle: isCircle (a::(getSubListToMember visited a p)) G
+  apply frontRepetitionInPathImpliesCircle
+  apply path
+  unfold isAcyclic at acyclic
+  specialize acyclic (a :: getSubListToMember visited a p)
+  exact absurd circle acyclic
+
+  simp [a_visited]
+  unfold isValid
+  simp
+  have a_mem: a ∈ G.vertices
+  apply isPath_front_member_graph path
+  specialize valid a a_mem
+  unfold locallyValid at valid
+  cases valid with
+  | inl valid =>
+    rcases valid with ⟨r,g,rP, grounding_r⟩
+    left
+    use r
+    constructor
+    apply rP
+    constructor
+    use g
+    rw [grounding_r, groundRuleEquality]
+    unfold groundRuleFromAtoms
+    simp
+
+    apply List.ext_get
+    rw [List.length_map, List.length_attach]
+    intro n h1 h2
+    rw [List.get_map]
+    simp
+    rw [rootOfExtractTreeStep]
+
+    rw [List.all₂_iff_forall]
+    simp
+    intro t ga ga_mem extract
+    rw [← extract]
+
+    specialize ih (height t)
+    have height_t_n: height t < n
+    rw [← h, ← extract]
+    apply extractTreeStepHeight
+    apply ga_mem
+    apply a_visited
+
+    specialize ih height_t_n ga (a::visited)
+
+    have path_ga: isPath (ga :: a :: visited) G
+    unfold isPath
+    simp
+    constructor
+    apply G.complete
+    apply a_mem
+    apply ga_mem
+    constructor
+    apply ga_mem
+    apply path
+
+    specialize ih path_ga
+    rw [← extract] at ih
+    simp at ih
+    apply ih
+  | inr dbCase =>
+    right
+    apply dbCase
+
+lemma verticesOfLocallyValidAcyclicGraphAreInProofTheoreticSemantics (P: program τ) (d: database τ)  (G: Graph (groundAtom τ)) (acyclic: isAcyclic G)  (valid: ∀ (a: groundAtom τ), a ∈ G.vertices → locallyValid P d a G): List.toSet G.vertices ⊆ proofTheoreticSemantics P d :=
+by
+  rw [Set.subset_def]
+  intro a a_mem
+  rw [← List.toSet_mem] at a_mem
+  unfold proofTheoreticSemantics
+  simp
+  use extractTreeStep a G [] (singletonPath a G a_mem)
+  constructor
+  apply rootOfExtractTreeStep
+  apply extractTreeStepValidProofTreeIffAllLocallyValidAndAcyclic
+  apply acyclic
+  apply valid
